Phoas_Graph.v
@@ -1,0 +1,76 @@
+Require Import List Arith Bool Maps FinFun Basics.
+
+Fixpoint f_maker (a b: nat) := fun (x:nat) => if beq_nat x a then b else 0.
+
+Definition edge_maker (x y:id) :=
+  match x,y with Id x1,Id y1 => 
+                 fun (a : id) => match a with Id a1 => Id ((f_maker x1 y1) a1) end
+  end.
+
+Definition V1 := Id 5.
+Definition V2 := Id 6.
+Definition V3 := Id 7.
+Definition V4 := Id 8.
+                    
+Definition f := edge_maker V1 V2.
+Definition g := edge_maker V2 V3.
+Definition h := edge_maker V3 V4.
+
+Eval compute in (f (Id 5)).     
+
+Definition nodeList := list id.
+Definition edgeList := list (id -> id).
+
+Check compose.
+
+Definition edge_compose (f g : id -> id) := compose g f.
+
+Definition f_inv := edge_maker (Id 6) (Id 5).
+Eval compute in  (edge_compose f f_inv) (Id 5).
+
+Eval compute in ((edge_compose (edge_compose f g) h) (Id 5)).     
+
+(*-------------------------------- not very useful, let's put more data in types*)
+
+Section phoas_graph.
+(* a universal constructor for nodes *)
+Inductive u (i : id) : Type :=
+  | U : u i.
+
+Definition v1 := U (Id 5).
+Check v1.
+
+Definition beq_U  {i j: id} (x : u i) (y : u j) := beq_id i j. 
+
+Definition edge_maker2 {i j: id} (x : u i) (y : u j) : u i -> u j :=
+  fun (a : u i) => U j.
+
+Definition edge_compose2 {i j k : id} (f : u i -> u j) (g : u j -> u k) :=
+  compose g f.
+
+Definition f1 := edge_maker2 (U V1) (U V2).
+Definition g1 := edge_maker2 (U V2) (U V3).
+Definition h1 := edge_maker2 (U V3) (U V4).
+
+Check f1.
+
+Check edge_compose2 (edge_compose2 f1 g1) h1.
+
+Definition nodeList2 := list (forall i:id, u i).
+Definition edgeList2 := list (forall i j:id, u i -> u j).
+
+
+(*better to use relations than functions, for pattern matching*)
+
+(*
+Fixpoint edgeListToAdjMap (el : edgeList2) (m : total_map edgeList2) : total_map edgeList2 :=
+  match el with
+  | nil => m
+  | hd :: tl => edgeListToAdjMap tl (t_update m i hd)
+  end.
+
+*)
+                
+  
+
+end phoas_graph
